Phi_System/Calculus_of_Programming.thy
@@ -51,7 +51,7 @@ definition PendingConstruction :: " 'ret::VALs proc
                                   \<Rightarrow> resource
                                   \<Rightarrow> assn
                                   \<Rightarrow> ('ret sem \<Rightarrow> assn)
-                                  \<Rightarrow> (ABNM sem \<Rightarrow> assn)
+                                  \<Rightarrow> (ABNM \<Rightarrow> assn)
                                   \<Rightarrow> bool "
     ("\<^bold>p\<^bold>e\<^bold>n\<^bold>d\<^bold>i\<^bold>n\<^bold>g _ \<^bold>o\<^bold>n _ [_]/ \<^bold>r\<^bold>e\<^bold>s\<^bold>u\<^bold>l\<^bold>t\<^bold>s \<^bold>i\<^bold>n _/ \<^bold>t\<^bold>h\<^bold>r\<^bold>o\<^bold>w\<^bold>s _" [1000,1000,1000,11,11] 10)
     where "PendingConstruction f s R S E \<longleftrightarrow> f s \<subseteq> \<S> (\<lambda>ret. INTERP_SPEC (R * S ret)) (\<lambda>ex. INTERP_SPEC (R * E ex))"
@@ -110,13 +110,14 @@ lemma \<phi>accept_proc:
   unfolding CurrentConstruction_def PendingConstruction_def bind_def subset_iff plus_fun_def
   apply clarsimp subgoal for s' s'' by (cases s'; simp; cases s''; simp add: ring_distribs; blast) .*)
 
+(*
 lemma \<phi>return_when_unreachable:
   \<open> \<^bold>p\<^bold>e\<^bold>n\<^bold>d\<^bold>i\<^bold>n\<^bold>g f \<^bold>o\<^bold>n s [R] \<^bold>r\<^bold>e\<^bold>s\<^bold>u\<^bold>l\<^bold>t\<^bold>s \<^bold>i\<^bold>n (\<lambda>_. T) \<^bold>t\<^bold>h\<^bold>r\<^bold>o\<^bold>w\<^bold>s E
 \<Longrightarrow> \<^bold>p\<^bold>e\<^bold>n\<^bold>d\<^bold>i\<^bold>n\<^bold>g (f \<ggreater> Return (sem undefined)) \<^bold>o\<^bold>n s [R] \<^bold>r\<^bold>e\<^bold>s\<^bold>u\<^bold>l\<^bold>t\<^bold>s \<^bold>i\<^bold>n (\<lambda>_. T) \<^bold>t\<^bold>h\<^bold>r\<^bold>o\<^bold>w\<^bold>s E\<close>
   for f :: \<open>unreachable proc\<close>
   unfolding CurrentConstruction_def PendingConstruction_def bind_def Return_def det_lift_def subset_iff
   apply clarsimp subgoal for s' s'' by (cases s'; simp; cases s''; simp add: ring_distribs; blast) .
-
+*)
 lemma \<phi>return_additional_unit:
   \<open> \<^bold>p\<^bold>e\<^bold>n\<^bold>d\<^bold>i\<^bold>n\<^bold>g f \<^bold>o\<^bold>n s [R] \<^bold>r\<^bold>e\<^bold>s\<^bold>u\<^bold>l\<^bold>t\<^bold>s \<^bold>i\<^bold>n T \<^bold>t\<^bold>h\<^bold>r\<^bold>o\<^bold>w\<^bold>s E
 \<Longrightarrow> \<^bold>p\<^bold>e\<^bold>n\<^bold>d\<^bold>i\<^bold>n\<^bold>g (f \<bind> (\<lambda>v. Return (\<phi>V_pair v \<phi>V_none))) \<^bold>o\<^bold>n s [R]
